Push out homework 3

src/01_Propositional_Logic/06_prop_logic_validation.lean
@@ -1,20 +1,13 @@
 
-#check tt = tt
-
-
-
 
 namespace cs6501
 
--- variables, indexed by natural numbers
 inductive prop_var : Type
 | mk (n : ℕ)
 
--- Abstract syntactic terms for unary operators
 inductive unop 
 | opNot
 
--- Abstract syntactic terms for binary operators
 inductive binop
 | opAnd
 | opOr
@@ -22,58 +15,49 @@ inductive binop
 | opIff
 | opXor
 
--- make constructor names globally visible
 open unop
 open binop
 
--- syntax
 inductive prop_expr : Type
 | pLit (b : bool)                         -- literal expressions
 | pVar (v: prop_var)                      -- variable expressions
--- | pNot (e : prop_expr)                    -- unary operator expression
 | pUnOp (op :unop) (e : prop_expr)                    -- unary operator expression
 | pBinOp (op : binop) (e1 e2 : prop_expr) -- binary operator expressions
 
 open prop_expr
 
-
-
--- notations (concrete syntax)
-def True := pLit tt
-def False := pLit ff
+notation ` ⊤ ` := pLit tt   -- Notation for True
+notation ` ⊥ ` := pLit ff   -- Notation for False
 notation (name := pVar) `[` v `]` :=  pVar v
 notation (name := pNot) ¬e := pUnOp opNot e
 notation (name := pAnd) e1 ∧ e2 :=  pBinOp opAnd e1 e2
 notation (name := pOr) e1 ∨ e2 :=  pBinOp opOr e1 e2
 precedence ` => `: 50                                      -- add operator precedence
-notation (name := pImp) e1 ` => `  e2 := pBinOp opImp e1 e2  -- bug fixed; add back quotes
+notation (name := pImp) e1 `=>`  e2 := pBinOp opImp e1 e2  -- bug fixed; add back quotes
 notation (name := pIff) e1 ↔ e2 := pBinOp opIff e1 e2
 notation (name := pXor) e1 ⊕ e2 := pBinOp opXor e1 e2
--- Let's not bother with notations for nand and nor at this point
 
 
 
 
--- Boolean implication operation (buggy!)
+-- implication 
+-- this specification is intentionally buggy
 def bimp : bool → bool → bool
 | tt tt := tt
 | tt ff := tt
 | ff tt := ff
 | ff ff := tt
 
--- Boolean biimplication operation
+-- bi-implication
 def biff : bool → bool → bool
 | tt tt := tt
 | tt ff := ff
 | ff tt := ff
 | ff ff := tt
 
-
--- interpretations of unary operators
 def un_op_sem : unop → (bool → bool)
 | opNot := bnot 
 
--- interpretations of binary operators
 def bin_op_sem : binop → (bool → bool → bool)
 | opAnd := band 
 | opOr  := bor
@@ -81,8 +65,6 @@ def bin_op_sem : binop → (bool → bool → bool)
 | opIff := biff
 | opXor := bxor
 
-
--- semantic evaluation (meaning of expressions)
 def pEval : prop_expr → (prop_var → bool) → bool
 | (pLit b)          i := b 
 | ([v])             i := i v                  -- our [] notation on the left
@@ -129,62 +111,15 @@ apply rfl,
 end 
 
 
--- tell Lean to explain given notations
-#print notation ¬ 
-#print notation ∧ 
-#print notation ↑
-
--- variables
-def v₀ := prop_var.mk 0
-def v₁ := prop_var.mk 1
-def v₂ := prop_var.mk 2
-
--- variable expressions
-def X := [v₀]
-def Y := [v₁]
-def Z := [v₂]
-
--- operator expressions
-def e1 := X ∧ Y
-def e2 := X ∨ Y
-def e3 := ¬Z
-def e4 := e1 => e2
-def e5 := e1 ↔ e1
-def e6 := X ⊕ ¬X
-
--- an interpretation
-def an_interp : prop_var → bool
-| (prop_var.mk 0) := tt -- X
-| (prop_var.mk 1) := ff -- Y
-| (prop_var.mk 2) := tt -- Z
-| _ := ff               -- any other variable
-
--- evaluation 
-#reduce pEval X an_interp  -- expect false
-#reduce pEval Y an_interp  -- expect false
-#reduce pEval e1 an_interp  -- expect false
-#reduce pEval (X => Y) an_interp  -- oops
-
--- applying theorem!
-#reduce and_commutes X Y an_interp
--- result is a proof that ff = ff
-
-
-
-
-
--- The proof that ∨ is commutative is basically identical to that for ∧
+-- ∨ is commutative
 def or_commutes : 
   ∀ (e1 e2 : prop_expr) 
     (i : prop_var → bool),
     (pEval (e1 ∨ e2) i) = (pEval (e2 ∨ e1) i) :=
 begin
--- Suppose e1 e2 and i are arbitrary expressions and interpretation
 assume e1 e2 i,
--- unfold definitions of pEval and bin_op_sem applied to their arguments
 unfold pEval,
 unfold bin_op_sem,
--- proof by simple case analysis on possible results of evaluating e1 and e2 under i
 cases (pEval e1 i),
 cases (pEval e2 i),
 apply rfl,
@@ -192,10 +127,9 @@ apply rfl,
 cases (pEval e2 i),
 apply rfl,
 apply rfl,
--- QED: By showing it's true for arbitrary e1/e2/i we've shown it's true for *all* 
 end 
 
--- Prove not is involutive
+-- negation (not) is involutive
 theorem not_involutive: ∀ e i, (pEval e i) = (pEval (¬¬e) i) :=
 begin
 assume e i,
@@ -205,6 +139,84 @@ cases (pEval e i),
 repeat { apply rfl },
 end
 
+-- implication is transitive
+theorem imp_trans : 
+  ∀ (e1 e2 e3 : prop_expr) (i : prop_var → bool),
+    (pEval (e1 => e2) i) = tt → 
+    (pEval (e2 => e3) i) = tt →
+    (pEval (e1 => e3) i) = tt :=
+begin
+unfold pEval,
+unfold bin_op_sem,
+assume e1 e2 e3 i h12 h23,
+cases (pEval e1 i),
+cases (pEval e2 i),
+cases (pEval e3 i),
+-- first 4 cases for e1
+assumption, --"exact rfl" will also work
+assumption,
+cases (pEval e3 i),
+assumption,
+assumption,
+-- second four cases for e1
+cases (pEval e2 i),
+cases (pEval e3 i),
+assumption,
+assumption,
+cases (pEval e3 i),
+assumption,
+assumption,
+end
+
+-- contrapositive: (X => Y) → (¬Y => ¬X)
+/-
+Example: if whenever it rains (X) the ground gets 
+wet (Y), then if the ground is NOT wet then is can't 
+have rained. Can we prove this principle to be valid
+in our logic? 
+-/
+theorem contrapos : 
+∀ (e1 e2 : prop_expr) 
+  (i : prop_var → bool),
+  (pEval (e1 => e2) i) = tt → 
+  (pEval (¬e2 => ¬e1)) i = tt :=
+begin
+assume e1 e2 i,
+unfold pEval,
+unfold un_op_sem bin_op_sem,    
+cases (pEval e1 i),
+cases (pEval e2 i),
+unfold bnot bimp,
+assume h,
+assumption,
+unfold bnot bimp,
+assume h,
+assumption,
+cases (pEval e2 i),
+unfold bnot bimp,
+assume h,
+assumption,
+unfold bnot bimp,
+assume h,
+assumption,
+end
+
+
+-- 1. X, Y ⊢ X ∧ Y            -- and_introduction
+-- 2. X ∧ Y ⊢ X               -- and_elimination_left
+-- 3. X ∧ Y ⊢ Y               -- and_elimination_right
+-- 4. ¬¬X ⊢ X                 -- negation elimination 
+-- 5. ¬(X ∧ ¬X)               -- no contradiction
+-- 6. X ⊢ X ∨ Y               -- or introduction left
+-- 7. Y ⊢ X ∨ Y               -- or introduction right
+-- 8. X ∨ Y, X → Z, Y → Z ⊢ Z -- or elimination
+-- 9. X → Y, Y → X ⊢ X ↔ Y    -- iff introduction
+-- 10. X ↔ Y ⊢ X → Y          -- iff elimination left
+-- 11. X ↔ Y ⊢ Y → X          -- iff elimination right
+-- 12. X → Y, X ⊢ Y           -- arrow elimination
+-- 13. X → Y, Y → Z ⊢ X → Z   -- transitivity of arrow 
+-- 14. X → Y ⊢ ¬Y → ¬X        -- contrapositive
+-- 15. ¬(X ∨ Y) ↔ ¬X ∧ ¬Y     -- DeMorgan 1 (¬ over ∨)
+-- 16. ¬(X ∧ Y) ↔ ¬X ∨ ¬Y     -- Demorgan 2 (¬ over ∧)
+
 end cs6501
-
-
