lean_source/01_Propositional_Logic/06_prop_logic_validation.lean
@@ -1,0 +1,353 @@
+/- TEXT:
+
+***************************
+Homework: Formal Validation
+***************************
+
+In class today, as evidenced by the developments in 
+the first section, below, we saw that it's not enough
+to prove a few theorems about a construction (here our
+syntax and semantics for propositional logic). One has
+to prove that a construction has *all* of the properties
+of the concept it's meant to represent.
+
+Improved Specification
+----------------------
+TEXT. -/
+
+
+-- QUOTE:
+namespace cs6501
+
+inductive prop_var : Type
+| mk (n : ℕ)
+
+inductive unop 
+| opNot
+
+inductive binop
+| opAnd
+| opOr
+| opImp
+| opIff
+| opXor
+
+open unop
+open binop
+
+inductive prop_expr : Type
+| pLit (b : bool)                         -- literal expressions
+| pVar (v: prop_var)                      -- variable expressions
+| pUnOp (op :unop) (e : prop_expr)                    -- unary operator expression
+| pBinOp (op : binop) (e1 e2 : prop_expr) -- binary operator expressions
+
+open prop_expr
+
+notation ` ⊤ ` := pLit tt   -- Notation for True
+notation ` ⊥ ` := pLit ff   -- Notation for False
+notation (name := pVar) `[` v `]` :=  pVar v
+notation (name := pNot) ¬e := pUnOp opNot e
+notation (name := pAnd) e1 ∧ e2 :=  pBinOp opAnd e1 e2
+notation (name := pOr) e1 ∨ e2 :=  pBinOp opOr e1 e2
+precedence ` => `: 50                                      -- add operator precedence
+notation (name := pImp) e1 `=>`  e2 := pBinOp opImp e1 e2  -- bug fixed; add back quotes
+notation (name := pIff) e1 ↔ e2 := pBinOp opIff e1 e2
+notation (name := pXor) e1 ⊕ e2 := pBinOp opXor e1 e2
+-- QUOTE.
+
+
+/- TEXT: 
+The *semantic domain* for our language is not only the
+Boolean values, but also the Boolean operations. We map
+variables to Boolean values via an *interpretation* and
+we define a fixed mapping of logical connectives (¬, ∧, 
+∨, etc.) to Boolean operations (bnot, band, bor, etc.)
+
+With these elementary semantic mappings in place we can
+finally now *any* propositional logical expression to 
+its (Boolean) meaning in a *compositional* manner, where
+the meaning of any compound expression is composed from
+the meanings of its parts, which we compute recursively,
+down to individual variables and connectives.
+
+The Lean standard libraries define some but not all 
+binary Boolean operations. We will thus start off in 
+this section by augmenting Lean's definitions of the
+Boolean operations with two more: for implication (we
+follow Lean naming conventions and call this bimp) and
+bi-implication (biff).
+TEXT. -/
+
+
+-- QUOTE:
+-- implication 
+-- this specification is intentionally buggy
+def bimp : bool → bool → bool
+| tt tt := tt
+| tt ff := tt
+| ff tt := ff
+| ff ff := tt
+
+-- bi-implication
+def biff : bool → bool → bool
+| tt tt := tt
+| tt ff := ff
+| ff tt := ff
+| ff ff := tt
+
+def un_op_sem : unop → (bool → bool)
+| opNot := bnot 
+
+def bin_op_sem : binop → (bool → bool → bool)
+| opAnd := band 
+| opOr  := bor
+| opImp := bimp
+| opIff := biff
+| opXor := bxor
+
+def pEval : prop_expr → (prop_var → bool) → bool
+| (pLit b)          i := b 
+| ([v])             i := i v                  -- our [] notation on the left
+| (pUnOp op e)      i := (un_op_sem op) (pEval e i)     -- our ¬ notation; Lean's bnot
+| (pBinOp op e1 e2) i := (bin_op_sem op) (pEval e1 i) (pEval e2 i) -- BUG FIXED :-)!
+-- QUOTE.
+
+
+/- TEXT:
+Formal Validation
+----------------- 
+
+The intended intuitive meaning of *and* in propositional
+logic is that both of its argument expresions are true,
+and that is all. To have this meaning requires that *and
+is commutative*. By that phrase we mean that the formula
+e1 ∧ e2 always means the same as e2 ∧ e1.
+
+To be precise we formalize this requirement with the
+following proposition, and_commutes, which we then prove.
+TEXT. -/
+
+-- QUOTE:
+-- proof of one key property: "commutativity of ∧" in the logic we've specified,, as required
+def and_commutes : 
+  ∀ (e1 e2 : prop_expr) 
+    (i : prop_var → bool),
+    (pEval (e1 ∧ e2) i) = (pEval (e2 ∧ e1) i) :=
+begin
+-- assume that e1 e2 and i are arbitrary
+assume e1 e2 i,
+
+-- unfold definition of pEval for given arguments
+unfold pEval,
+
+-- unfold definition of bin_op_sem
+unfold bin_op_sem,
+
+-- case analysis on Boolean value (pEval e1 i)
+cases (pEval e1 i),
+
+-- within first case, nested case analysis on (pEval e2 i)
+cases (pEval e2 i),
+
+-- goal proved by reflexivity of equality
+apply rfl,
+
+-- second case for (pEval e2 i) within first case for  (pEval e1 i)
+apply rfl,
+
+-- onto second case for (pEval e1 i)
+-- again nested case analysis on (pEval e2 i)
+cases (pEval e2 i),
+
+-- and both cases are again true by reflexivity of equality 
+apply rfl,
+apply rfl,
+-- QED
+end 
+-- QUOTE.
+
+/- TEXT: 
+Exercises
+---------
+
+1. Formally state and prove that in our language, or (∨) is commutative (1 minute!)
+2. Formally state and prove that in our language, not (¬) is involutive (a few minutes). 
+   Hints: Put parens around (¬¬e). Open the Lean infoview with CTRL/CMD-SHIFT-RETURN/ENTER.
+   If you get hung up on Lean syntax, ask a friend (or instructor) for help to get unstuck.
+
+Solutions
+---------
+TEXT. -/
+
+-- QUOTE:
+-- ∨ is commutative
+def or_commutes : 
+  ∀ (e1 e2 : prop_expr) 
+    (i : prop_var → bool),
+    (pEval (e1 ∨ e2) i) = (pEval (e2 ∨ e1) i) :=
+begin
+assume e1 e2 i,
+unfold pEval,
+unfold bin_op_sem,
+cases (pEval e1 i),
+cases (pEval e2 i),
+apply rfl,
+apply rfl,
+cases (pEval e2 i),
+apply rfl,
+apply rfl,
+end 
+
+-- negation (not) is involutive
+theorem not_involutive: ∀ e i, (pEval e i) = (pEval (¬¬e) i) :=
+begin
+assume e i,
+unfold pEval,
+unfold un_op_sem,
+cases (pEval e i),
+repeat { apply rfl },
+end
+
+-- implication is transitive
+theorem imp_trans : 
+  ∀ (e1 e2 e3 : prop_expr) (i : prop_var → bool),
+    (pEval (e1 => e2) i) = tt → 
+    (pEval (e2 => e3) i) = tt →
+    (pEval (e1 => e3) i) = tt :=
+begin
+unfold pEval,
+unfold bin_op_sem,
+assume e1 e2 e3 i h12 h23,
+cases (pEval e1 i),
+cases (pEval e2 i),
+cases (pEval e3 i),
+-- first 4 cases for e1
+assumption, --"exact rfl" will also work
+assumption,
+cases (pEval e3 i),
+assumption,
+assumption,
+-- second four cases for e1
+cases (pEval e2 i),
+cases (pEval e3 i),
+assumption,
+assumption,
+cases (pEval e3 i),
+assumption,
+assumption,
+end
+
+-- contrapositive: (X => Y) → (¬Y => ¬X)
+/-
+Example: if whenever it rains (X) the ground gets 
+wet (Y), then if the ground is NOT wet then is can't 
+have rained. Can we prove this principle to be valid
+in our logic? 
+-/
+theorem contrapos : 
+∀ (e1 e2 : prop_expr) 
+  (i : prop_var → bool),
+  (pEval (e1 => e2) i) = tt → 
+  (pEval (¬e2 => ¬e1)) i = tt :=
+begin
+assume e1 e2 i,
+unfold pEval,
+unfold un_op_sem bin_op_sem,    
+cases (pEval e1 i),
+cases (pEval e2 i),
+unfold bnot bimp,
+assume h,
+assumption,
+unfold bnot bimp,
+assume h,
+assumption,
+cases (pEval e2 i),
+unfold bnot bimp,
+assume h,
+assumption,
+unfold bnot bimp,
+assume h,
+assumption,
+end
+-- QUOTE.
+
+/- TEXT:
+Homework
+--------
+
+Wow, we know that bimp is buggy and yet we were able
+to prove both of these properties about it. Right! To
+fully validate, and thus *know for sure* that our logic 
+correctly simulates propositional logic, we need to prove
+that *all* of the essential properties of the logic hold
+for our representation. 
+
+Here's a set of rules that's more complete. You job is 
+to formally state each rule then prove that it holds in 
+our logic. As you do this, identify the rule(s) that 
+can't be proved due to the fault in our specification, 
+bimp, of the Boolean implication operation.
+
+We present these rules in the form of sequents. Express 
+each of the rules in our logic by replacing turnstiles
+(⊢) with implies (=>), and commas (,) with and (∧). Use
+parenthesis pairs to specify grouping explicitly if you're
+unsure of precendence and/or associativity. Then prove 
+that each formula is true, for *all* expressions, X, Y, 
+and Z, and *all* interpretations/assignments-of-values, 
+*i,* for X, Y, and Z.
+TEXT. -/
+
+-- QUOTE:
+-- 1. X, Y ⊢ X ∧ Y            -- and_introduction
+-- 2. X ∧ Y ⊢ X               -- and_elimination_left
+-- 3. X ∧ Y ⊢ Y               -- and_elimination_right
+-- 4. ¬¬X ⊢ X                 -- negation elimination 
+-- 5. ¬(X ∧ ¬X)               -- no contradiction
+-- 6. X ⊢ X ∨ Y               -- or introduction left
+-- 7. Y ⊢ X ∨ Y               -- or introduction right
+-- 8. X ∨ Y, X → Z, Y → Z ⊢ Z -- or elimination
+-- 9. X → Y, Y → X ⊢ X ↔ Y    -- iff introduction
+-- 10. X ↔ Y ⊢ X → Y          -- iff elimination left
+-- 11. X ↔ Y ⊢ Y → X          -- iff elimination right
+-- 12. X → Y, X ⊢ Y           -- arrow elimination
+-- 13. X → Y, Y → Z ⊢ X → Z   -- transitivity of arrow 
+-- 14. X → Y ⊢ ¬Y → ¬X        -- contrapositive
+-- 15. ¬(X ∨ Y) ↔ ¬X ∧ ¬Y     -- DeMorgan 1 (¬ over ∨)
+-- 16. ¬(X ∧ Y) ↔ ¬X ∨ ¬Y     -- Demorgan 2 (¬ over ∧)
+-- QUOTE.
+
+/- TEXT:
+In the style we've developed, formally state and prove 
+that our logic and semantics has each of the properties, 
+1, 2, 4, 5, 6, 8, 9, 10, 12, and 15. Identify any rules 
+that fail to be provable due to the injected bug in bimp.
+
+Use Lean's *theorem* directive to give names to proofs. 
+as names for your proofs, use the names in the comments
+after each rule (adding missing underscores as needed).
+
+To do this part of the assignment, make a copy of this
+file from the class repo and add the statement and proof
+of each theorem below. You will turn in the file with these
+proofs included in the given order at the end of the file.
+
+This isn't a comprehensive list of properties. We lack
+rules for ⊤ and ⊥ (formerly True, False; still terms 
+that invariably evaluate to true (tt) and false (ff).
+There are rules that explain, for example, that ⊤ ∧ e 
+is equivalent to e; ⊥ ∧ e is invariably false; ⊥ or e 
+is equivalent to e; and ⊤ ∨ e is invariably true. Go 
+ahead and prove these propositions as well if you just
+can't stop proving! (optional :-).
+
+Try to do all or at least most of this assignment on 
+your own. Feel free to ask for or give help on minor
+matters, e.g., of Lean syntax, or if some concept isn't
+yet clear enough. Discussing such issues is constructive. 
+I skipped over properties whose proofs look almost just
+like those for closely related properties.
+TEXT. -/
+-- QUOTE:
+end cs6501
+-- QUOTE.
