src/01_Propositional_Logic/solutions/solutions_05_prop_logic_properties.lean
@@ -1,1 +1,3 @@
 
+#check tt = tt
+
