source/01_Propositional_Logic.rst
@@ -6,3 +6,4 @@
 .. include:: 01_Propositional_Logic/03_prop_logic_syn_sem.inc
 .. include:: 01_Propositional_Logic/04_prop_logic_syn_sem.inc
 .. include:: 01_Propositional_Logic/05_prop_logic_properties.inc
+.. include:: 01_Propositional_Logic/06_prop_logic_validation.inc
